More var -> positive code

theories/Infra/Fresh.v
@@ -1,121 +1,312 @@
 Require Import CSet Le Arith.Compare_dec.
 Require Import Plus Util Map Get Take LengthEq SafeFirst.
-Require Export StableFresh.
+Require Export PidgeonHole StableFresh.
 
 Set Implicit Arguments.
 
-Definition fresh (s : set nat) : nat :=
-  S(fold max s 0).
 
-Lemma max_transpose
-  : transpose eq max.
+Class LeastFresh V `{NaturalRepresentation V} :=
+  {
+    least_fresh :> set V -> V;
+    least_fresh_spec : forall G, least_fresh G ∉ G;
+    least_fresh_least : forall G y, _lt y (least_fresh G) -> y ∈ G;
+    least_fresh_ext : forall G G', G [=] G' -> least_fresh G = least_fresh G'
+  }.
+
+Arguments LeastFresh V {H} {H0}.
+
+Definition nr_max X `{OrderedType X} (x y:X) :=
+  if [_lt x y] then y else x.
+
+Arguments nr_max {X} {H} x y.
+
+Instance nr_max_eq_proper X `{OrderedType X}
+  : Proper (_eq ==> _eq ==> _eq) nr_max.
 Proof.
-  hnf; intros. rewrite Max.max_assoc. rewrite (Max.max_comm x).
-  rewrite Max.max_assoc. reflexivity.
+  unfold Proper, respectful; intros.
+  unfold nr_max. repeat cases; eauto.
+  exfalso. eapply NOTCOND. rewrite <- H1, <- H0. eauto.
+  exfalso. eapply NOTCOND. rewrite H1, H0. eauto.
 Qed.
 
-Lemma fresh_spec' (G:set nat)
-  : forall (x:nat), x ∈ G -> x <= fold max G 0.
+Lemma nr_max_sym X `{OrderedType X} (x y:X)
+  : nr_max x y === nr_max y x.
 Proof.
-  pattern G. pattern (fold max G 0). eapply fold_rec; intros.
-  - cset_tac.
-  - eapply H1 in H3. destruct H3.
-    + pattern (fold max s'' 0). rewrite fold_2; eauto.
-      * rewrite H3. pose proof (Max.le_max_l x0 (fold max s' 0)).
-        eapply H4.
-      * intuition.
-      * eapply max_transpose.
-    + pattern (fold max s'' 0). rewrite fold_2; eauto.
-      * pose proof (Max.le_max_r x (fold max s' 0)).
-        specialize (H2 _ H3). unfold max in H2. rewrite <- H4. eapply H2.
-      * intuition.
-      * eapply max_transpose.
+  unfold nr_max; repeat cases; eauto; exfalso.
+  - assert (_lt x x) by (etransitivity; eauto).
+    eapply OrderedType.StrictOrder_Irreflexive in H0; eauto.
+  - admit.
+Admitted.
+
+Lemma nr_max_assoc X `{OrderedType X} (x y z:X)
+  : nr_max x (nr_max y z) === nr_max (nr_max x y) z.
+Proof.
+  unfold nr_max; repeat cases; eauto; exfalso; eauto.
+  - cases in COND0; eauto.
+  - cases in NOTCOND; cases in COND; eauto.
+    eapply NOTCOND; etransitivity; eauto.
+    admit.
+  - cases in NOTCOND; eauto.
+Admitted.
+
+Class NaturalRepresentationSucc V `{NaturalRepresentation V} :=
+  {
+    succ : V -> V;
+    succ_asNat : forall x, asNat (succ x) = S (asNat x);
+    succ_ofNat : forall n:nat, succ (ofNat n) === ofNat (S n);
+    respect_lt :> Proper (_lt ==> _lt) succ;
+    respect_eq :> Proper (_eq ==> _eq) succ
+  }.
+
+
+Section LeastFresh.
+  Variable V : Type.
+  Context `{NaturalRepresentationSucc V}.
+
+  Definition fresh (s : set V) : V :=
+    succ (fold nr_max s (ofNat 0)).
+
+  Lemma max_transpose
+    : transpose _eq nr_max.
+  Proof.
+    hnf; intros.
+    rewrite nr_max_sym. rewrite <- nr_max_assoc.
+    setoid_rewrite nr_max_sym at 2. reflexivity.
+  Qed.
+
+  Lemma fold_max_lt (G:set V)
+    : forall (x:V), x ∈ G -> _lt x (succ (fold nr_max G (ofNat 0))).
+  Proof.
+    pattern G. pattern (fold nr_max G (ofNat 0)). eapply fold_rec; intros.
+    - cset_tac.
+    - eapply H4 in H6. destruct H6.
+      + rewrite fold_2; eauto.
+        * rewrite <- H6. admit.
+        * eapply nr_max_eq_proper.
+        * eapply max_transpose.
+      + rewrite fold_2; eauto.
+        * (*pose proof (Max.le_max_r x (fold max s' 0)).
+          specialize (H2 _ H3). unfold max in H2. rewrite <- H4. eapply H2.*)
+          admit.
+        * eapply nr_max_eq_proper.
+        * eapply max_transpose.
+  Admitted.
+
+  Lemma fresh_spec G : fresh G ∉ G.
+  Proof.
+    intro. unfold fresh in H2.
+    pose proof (fold_max_lt H2).
+    eapply lt_antirefl in H3; eauto.
+  Qed.
+
+  Lemma fresh_variable_always_exists (lv:set V) n
+    : safe (fun x => x ∉ lv) n.
+  Proof.
+    - decide (n > fold max lv 0).
+      + econstructor; intro.
+        exploit fresh_spec'; eauto. omega.
+      + eapply safe_antitone with (n:=S (fold max lv 0)); [|omega].
+        econstructor. intro. exploit fresh_spec'; eauto; omega.
+  Qed.
+
+  Definition least_fresh (lv:set nat) : nat.
+    refine (@safe_first (fun x => x ∉ lv) _ 0 _).
+    - eapply fresh_variable_always_exists.
+  Defined.
+
+  Lemma all_in_lv_cardinal (lv:set nat) n
+    : (forall m : nat, m < n -> m \In lv) -> cardinal lv >= n.
+  Proof.
+    general induction n; simpl.
+    - omega.
+    - exploit (IHn (lv \ singleton n)).
+      + intros. cset_tac'; omega.
+      + assert (lv [=] {n; lv \ singleton n }). {
+          exploit (H (n)); eauto.
+          cset_tac.
+        }
+        rewrite H1.
+        assert (n ∉ lv \ singleton n) by cset_tac.
+        erewrite cardinal_2; eauto. omega.
+  Qed.
+
+  Lemma neg_pidgeon_hole (lv:set nat)
+    : (forall m : nat, m <= cardinal lv -> m \In lv) -> False.
+  Proof.
+    intros. exploit (@all_in_lv_cardinal lv (S (cardinal lv))).
+    intros; eapply H; eauto. omega. omega.
+  Qed.
+
+  Lemma least_fresh_full_spec G
+    : least_fresh G ∉ G
+      /\ least_fresh G <= cardinal G
+      /\ forall m, m < least_fresh G -> m ∈ G.
+  Proof.
+    unfold least_fresh.
+    eapply safe_first_spec with (I:= fun n => le n (cardinal G) /\ forall m, m < n -> m ∈ G).
+    - intros; dcr.
+      assert (n ∈ G) by cset_tac; clear H0.
+      split.
+      + eapply all_in_lv_cardinal.
+        intros. decide (m = n); subst; eauto.
+        eapply H2. omega.
+      + intros. decide (m = n); subst; eauto.
+        eapply H2; omega.
+    - intuition.
+    - split; intros; omega.
+  Qed.
+
+  Lemma least_fresh_ext (G G':set nat)
+    : G [=] G'
+      -> least_fresh G = least_fresh G'.
+  Proof.
+    intros. unfold least_fresh.
+    eapply safe_first_ext; eauto.
+    split; intros.
+    - rewrite <- H; eauto.
+    - rewrite H; eauto.
+  Qed.
+
+End LeastFreshNat.
+
+Instance LeastFreshNat : LeastFresh nat :=
+  {
+    least_fresh := LeastFreshNat.least_fresh
+  }.
+Proof.
+  - intros. eapply LeastFreshNat.least_fresh_full_spec.
+  - intros. eapply LeastFreshNat.least_fresh_full_spec; eauto.
+  - intros. eapply LeastFreshNat.least_fresh_ext; eauto.
 Qed.
 
-Lemma fresh_spec G : fresh G ∉ G.
+
+Module LeastFreshPositive.
+  Definition fresh (s : set positive) : positive :=
+    S(fold max s 0).
+
+  Lemma max_transpose
+    : transpose eq max.
+  Proof.
+    hnf; intros. rewrite Max.max_assoc. rewrite (Max.max_comm x).
+    rewrite Max.max_assoc. reflexivity.
+  Qed.
+
+  Lemma fresh_spec' (G:set nat)
+    : forall (x:nat), x ∈ G -> x <= fold max G 0.
+  Proof.
+    pattern G. pattern (fold max G 0). eapply fold_rec; intros.
+    - cset_tac.
+    - eapply H1 in H3. destruct H3.
+      + pattern (fold max s'' 0). rewrite fold_2; eauto.
+        * rewrite H3. pose proof (Max.le_max_l x0 (fold max s' 0)).
+          eapply H4.
+        * intuition.
+        * eapply max_transpose.
+      + pattern (fold max s'' 0). rewrite fold_2; eauto.
+        * pose proof (Max.le_max_r x (fold max s' 0)).
+          specialize (H2 _ H3). unfold max in H2. rewrite <- H4. eapply H2.
+        * intuition.
+        * eapply max_transpose.
+  Qed.
+
+  Lemma fresh_spec G : fresh G ∉ G.
+  Proof.
+    intro. unfold fresh in H.
+    pose proof (fresh_spec' H). omega.
+  Qed.
+
+  Lemma fresh_variable_always_exists (lv:set nat) n
+    : safe (fun x => x ∉ lv) n.
+  Proof.
+    - decide (n > fold max lv 0).
+      + econstructor; intro.
+        exploit fresh_spec'; eauto. omega.
+      + eapply safe_antitone with (n:=S (fold max lv 0)); [|omega].
+        econstructor. intro. exploit fresh_spec'; eauto; omega.
+  Qed.
+
+  Definition least_fresh (lv:set nat) : nat.
+    refine (@safe_first (fun x => x ∉ lv) _ 0 _).
+    - eapply fresh_variable_always_exists.
+  Defined.
+
+  Lemma all_in_lv_cardinal (lv:set nat) n
+    : (forall m : nat, m < n -> m \In lv) -> cardinal lv >= n.
+  Proof.
+    general induction n; simpl.
+    - omega.
+    - exploit (IHn (lv \ singleton n)).
+      + intros. cset_tac'; omega.
+      + assert (lv [=] {n; lv \ singleton n }). {
+          exploit (H (n)); eauto.
+          cset_tac.
+        }
+        rewrite H1.
+        assert (n ∉ lv \ singleton n) by cset_tac.
+        erewrite cardinal_2; eauto. omega.
+  Qed.
+
+  Lemma neg_pidgeon_hole (lv:set nat)
+    : (forall m : nat, m <= cardinal lv -> m \In lv) -> False.
+  Proof.
+    intros. exploit (@all_in_lv_cardinal lv (S (cardinal lv))).
+    intros; eapply H; eauto. omega. omega.
+  Qed.
+
+  Lemma least_fresh_full_spec G
+    : least_fresh G ∉ G
+      /\ least_fresh G <= cardinal G
+      /\ forall m, m < least_fresh G -> m ∈ G.
+  Proof.
+    unfold least_fresh.
+    eapply safe_first_spec with (I:= fun n => le n (cardinal G) /\ forall m, m < n -> m ∈ G).
+    - intros; dcr.
+      assert (n ∈ G) by cset_tac; clear H0.
+      split.
+      + eapply all_in_lv_cardinal.
+        intros. decide (m = n); subst; eauto.
+        eapply H2. omega.
+      + intros. decide (m = n); subst; eauto.
+        eapply H2; omega.
+    - intuition.
+    - split; intros; omega.
+  Qed.
+
+  Lemma least_fresh_ext (G G':set nat)
+    : G [=] G'
+      -> least_fresh G = least_fresh G'.
+  Proof.
+    intros. unfold least_fresh.
+    eapply safe_first_ext; eauto.
+    split; intros.
+    - rewrite <- H; eauto.
+    - rewrite H; eauto.
+  Qed.
+
+End LeastFreshNat.
+
+Instance LeastFreshNat : LeastFresh nat :=
+  {
+    least_fresh := LeastFreshNat.least_fresh
+  }.
 Proof.
-  intro. unfold fresh in H.
-  pose proof (fresh_spec' H). omega.
+  - intros. eapply LeastFreshNat.least_fresh_full_spec.
+  - intros. eapply LeastFreshNat.least_fresh_full_spec; eauto.
+  - intros. eapply LeastFreshNat.least_fresh_ext; eauto.
 Qed.
 
-Lemma fresh_variable_always_exists (lv:set nat) n
-: safe (fun x => x ∉ lv) n.
-Proof.
-  - decide (n > fold max lv 0).
-    + econstructor; intro.
-      exploit fresh_spec'; eauto. omega.
-    + eapply safe_antitone with (n:=S (fold max lv 0)); [|omega].
-      econstructor. intro. exploit fresh_spec'; eauto; omega.
-Qed.
-
-Definition least_fresh (lv:set nat) : nat.
-  refine (@safe_first (fun x => x ∉ lv) _ 0 _).
-  - eapply fresh_variable_always_exists.
-Defined.
-
-Lemma all_in_lv_cardinal (lv:set nat) n
-: (forall m : nat, m < n -> m \In lv) -> cardinal lv >= n.
-Proof.
-  general induction n; simpl.
-  - omega.
-  - exploit (IHn (lv \ singleton n)).
-    + intros. cset_tac'; omega.
-    + assert (lv [=] {n; lv \ singleton n }). {
-        exploit (H (n)); eauto.
-        cset_tac.
-      }
-      rewrite H1.
-      assert (n ∉ lv \ singleton n) by cset_tac.
-      erewrite cardinal_2; eauto. omega.
-Qed.
-
-Lemma neg_pidgeon_hole (lv:set nat)
-: (forall m : nat, m <= cardinal lv -> m \In lv) -> False.
-Proof.
-  intros. exploit (@all_in_lv_cardinal lv (S (cardinal lv))).
-  intros; eapply H; eauto. omega. omega.
-Qed.
-
-Lemma least_fresh_full_spec G
-  : least_fresh G ∉ G
-    /\ least_fresh G <= cardinal G
-    /\ forall m, m < least_fresh G -> m ∈ G.
-Proof.
-  unfold least_fresh.
-  eapply safe_first_spec with (I:= fun n => le n (cardinal G) /\ forall m, m < n -> m ∈ G).
-  - intros; dcr.
-    assert (n ∈ G) by cset_tac; clear H0.
-    split.
-    + eapply all_in_lv_cardinal.
-      intros. decide (m = n); subst; eauto.
-      eapply H2. omega.
-    + intros. decide (m = n); subst; eauto.
-      eapply H2; omega.
-  - intuition.
-  - split; intros; omega.
-Qed.
-
-Lemma least_fresh_ext (G G':set nat)
-: G [=] G'
-  -> least_fresh G = least_fresh G'.
-Proof.
-  intros. unfold least_fresh.
-  eapply safe_first_ext; eauto.
-  split; intros.
-  - rewrite <- H; eauto.
-  - rewrite H; eauto.
-Qed.
-
+(*
 Lemma least_fresh_spec G
 : least_fresh G ∉ G.
 Proof.
   eapply least_fresh_full_spec.
 Qed.
 
-Lemma least_fresh_small G
+Lemma least_fresh_small (G:set nat)
 : least_fresh G <= cardinal G.
 Proof.
-  eapply least_fresh_full_spec.
+  unfold least_fresh. simpl.
+  eapply LeastFreshNat.least_fresh_full_spec.
 Qed.
 
 Lemma least_fresh_smallest G
@@ -132,18 +323,20 @@ Lemma fresh_stable_spec G x
 Proof.
   unfold fresh_stable. cases; eauto using fresh_spec.
 Qed.
+*)
 
 Section FreshList.
+  Variable V : Type.
+  Context `{OrderedType V}.
+  Variable fresh : set V -> V.
 
-  Variable fresh : set nat -> nat.
-
-  Fixpoint fresh_list (G:set nat) (n:nat) : list nat :=
+  Fixpoint fresh_list (G:set V) (n:nat) : list V :=
     match n with
       | 0 => nil
       | (S n) => let y := fresh G in y::fresh_list {y;G} n
     end.
 
-  Lemma fresh_list_length (G:set nat) n
+  Lemma fresh_list_length (G:set V) n
   : length (fresh_list G n) = n.
   Proof.
     general induction n; eauto. simpl. f_equal; eauto.
@@ -151,73 +344,74 @@ Section FreshList.
 
   Hypothesis fresh_spec : forall G, fresh G ∉ G.
 
-  Definition fresh_set (G:set nat) L : set nat :=
+  Definition fresh_set (G:set V) L : set V :=
     of_list (fresh_list G L).
 
-  Lemma fresh_list_spec : forall (G:set nat) n, disj (of_list (fresh_list G n)) G.
+  Lemma fresh_list_spec : forall (G:set V) n, disj (of_list (fresh_list G n)) G.
   Proof.
     intros. general induction n; simpl; intros; eauto.
     - hnf; intros. cset_tac'.
-      + specialize (H ({fresh G; G})).
-        eapply H; eauto.
+      + rewrite <- H2 in H1. eauto.
+      + specialize (H0 ({fresh G; G})).
+        eapply H0; eauto.
         cset_tac.
   Qed.
 
   Lemma fresh_set_spec
-  : forall (G:set nat) L, disj (fresh_set G L) G.
+  : forall (G:set V) L, disj (fresh_set G L) G.
   Proof.
     unfold fresh_set. eapply fresh_list_spec.
   Qed.
 
-  Lemma fresh_list_nodup (G: set nat) n
+  Lemma fresh_list_nodup (G: set V) n
     : NoDupA eq (fresh_list G n).
   Proof.
     general induction n; simpl; eauto.
     econstructor; eauto. intro.
     eapply fresh_list_spec.
-    eapply InA_in. eapply H.
-    cset_tac; eauto.
+    eapply InA_eq_of_list; eauto.
+    cset_tac.
+  Qed.
+
+  Lemma fresh_list_ext n G G'
+    : (forall G G', G [=] G' -> fresh G = fresh G')
+      -> G [=] G'
+      -> fresh_list G n = fresh_list G' n.
+  Proof.
+    intros EXT EQ. general induction n; simpl.
+    - reflexivity.
+    - f_equal. eauto.
+      eapply IHn; eauto.
+      erewrite EXT, EQ; eauto; reflexivity.
   Qed.
 
 End FreshList.
 
-
-Lemma fresh_list_ext n G G' f
-  : (forall G G', G [=] G' -> f G = f G')
-    -> G [=] G'
-    -> fresh_list f G n = fresh_list f G' n.
-Proof.
-  intros EXT EQ. general induction n; simpl.
-  - reflexivity.
-  - f_equal; eauto using least_fresh_ext.
-    eapply IHn; eauto.
-    erewrite EXT, EQ; eauto; reflexivity.
-Qed.
-
-
 Hint Resolve fresh_list_length : len.
 
 
-Lemma least_fresh_list_small G n
-: forall i x, get (fresh_list least_fresh G n) i x -> x < cardinal G + n.
+Lemma least_fresh_list_small X `{LeastFresh X} (G:set X) n
+: forall i x, get (fresh_list least_fresh G n) i x -> asNat x < cardinal G + n.
 Proof.
   general induction n; simpl in *; isabsurd.
-  - inv H.
-    + exploit (least_fresh_small G). omega.
+  - invc H2.
+    + clear IHn.
+      pose proof (least_fresh_least G).
+      eapply all_in_lv_cardinal in H2.
+      omega.
     + exploit IHn; eauto.
-      erewrite cardinal_2 with (s:=G) in H0. omega.
+      erewrite cardinal_2 with (s:=G) in H2. omega.
       eapply (least_fresh_spec). cset_tac.
 Qed.
 
-Lemma least_fresh_list_ext n G G'
+Lemma least_fresh_list_ext X `{LeastFresh X}  n (G:set X) G'
   : G [=] G'
     -> fresh_list least_fresh G n = fresh_list least_fresh G' n.
 Proof.
-  intros EQ. general induction n; simpl.
-  - reflexivity.
-  - f_equal; eauto using least_fresh_ext.
-    eapply IHn.
-    erewrite least_fresh_ext, EQ; eauto; reflexivity.
+  intros.
+  eapply fresh_list_ext; eauto.
+  eapply least_fresh_spec.
+  eapply least_fresh_ext.
 Qed.
 
 Fixpoint nats_up_to (n:nat) :=
@@ -252,7 +446,7 @@ Lemma least_fresh_list_small_nats_up_to G n
 Proof.
   eapply get_in_incl; intros.
   eapply in_nats_up_to.
-  eapply least_fresh_list_small; eauto.
+  eapply least_fresh_list_small in H; eauto.
 Qed.
 
 Lemma nats_up_to_max n m
@@ -276,16 +470,6 @@ Proof.
         omega.
 Qed.
 
-Lemma inverse_on_update_fresh_list (D:set nat) (Z:list nat) (ϱ ϱ' : nat -> nat)
- : inverse_on (D \ of_list Z) ϱ ϱ'
-  -> inverse_on D (update_with_list Z (fresh_list fresh (lookup_set ϱ (D \ of_list Z)) (length Z)) ϱ)
-                 (update_with_list (fresh_list fresh (lookup_set ϱ (D \ of_list Z)) ((length Z))) Z ϱ').
-Proof.
-  intros. eapply inverse_on_update_fresh; eauto. intros.
-  eapply fresh_list_nodup, fresh_spec. eauto with len.
-  eapply fresh_list_spec, fresh_spec.
-Qed.
-
 Lemma nats_up_to_in x i
   : x < i <-> x ∈ nats_up_to i.
 Proof.
@@ -297,3 +481,15 @@ Proof.
       -- cset_tac'. eapply H0. omega.
       -- cset_tac'.
 Qed.
+
+(*
+Lemma inverse_on_update_fresh_list (D:set nat) (Z:list nat) (ϱ ϱ' : nat -> nat)
+ : inverse_on (D \ of_list Z) ϱ ϱ'
+  -> inverse_on D (update_with_list Z (fresh_list fresh (lookup_set ϱ (D \ of_list Z)) (length Z)) ϱ)
+                 (update_with_list (fresh_list fresh (lookup_set ϱ (D \ of_list Z)) ((length Z))) Z ϱ').
+Proof.
+  intros. eapply inverse_on_update_fresh; eauto. intros.
+  eapply fresh_list_nodup, fresh_spec. eauto with len.
+  eapply fresh_list_spec, fresh_spec.
+Qed.
+ *)
