theories/Equiv/CtxEq.v
@@ -272,7 +272,8 @@ Proof.
         eapply star2_refl.
       * split.
         -- hnf; intros. lud; eauto.
-           eapply H3; eauto. rewrite H1 in H5. cset_tac.
+           ++ rewrite e. reflexivity.
+           ++ eapply H3; eauto. rewrite H1 in H5. cset_tac.
         -- eapply agree_on_update_dead. rewrite H1. cset_tac; intuition.
            eapply agree_on_incl; eauto. eapply H3; eauto.
            rewrite H1. cset_tac.
